Change proof to extrinsic style in Raindrop

raindrops/Raindrops.fst
@@ -1,7 +1,19 @@
 module Raindrops
 open Bridge
 
-module I = FStar.Int
+(*
+    If the number contains 3 as a factor, output 'Pling'.
+    If the number contains 5 as a factor, output 'Plang'.
+    If the number contains 7 as a factor, output 'Plong'.
+    If the number does not contain 3, 5, or 7 as a factor, just pass the number's digits straight through.
+*)
+val raindrop : native_int -> string
+let raindrop n = match of_int n with
+    | n when n % 3 <> 0 && n % 5 <> 0 && n % 7 <> 0 -> string_of_int n
+    | n -> (if n % 3 = 0 then "Pling" else "")
+            ^ (if n % 5 = 0 then "Plang" else "")
+            ^ (if n % 7 = 0 then "Plong" else "")
+
 module S = FStar.String
 
 val string_of_int_return_not_empty_string: (n:int) -> Lemma (ensures S.length (string_of_int n) <> 0) [SMTPat (string_of_int n)]
@@ -10,29 +22,16 @@ let string_of_int_return_not_empty_string = admit()
 val strcat_add_length: (s1:string) -> (s2:string) -> Lemma (ensures (S.length s1) + (S.length s2) = (S.length (s1 ^ s2))) [SMTPat (s1 ^ s2)]
 let strcat_add_length = admit()
 
-// TODO: I don't know how to prove a literal
-val literal_to_string: string -> string
-let literal_to_string s = s
-
-val empty_string_length_is_zero: (s:string) -> Lemma (requires s = "") (ensures S.length (literal_to_string s) = 0) [SMTPat (literal_to_string s)]
+val empty_string_length_is_zero: (s:string) -> Lemma (requires s = "") (ensures S.length s = 0)
 let empty_string_length_is_zero = admit()
 
-val not_empty_string_length_is_pos: (s:string) -> Lemma (requires s <> "") (ensures S.length (literal_to_string s) > 0) [SMTPat (literal_to_string s)]
+val not_empty_string_length_is_pos: (s:string) -> Lemma (requires s <> "") (ensures S.length s > 0)
 let not_empty_string_length_is_pos = admit()
 
-(*
-    If the number contains 3 as a factor, output 'Pling'.
-    If the number contains 5 as a factor, output 'Plang'.
-    If the number contains 7 as a factor, output 'Plong'.
-    If the number does not contain 3, 5, or 7 as a factor, just pass the number's digits straight through.
-*)
-val raindrop : native_int -> (sound:string{S.length sound > 0})
-let raindrop n =
-    let n = of_int n in
-    if n % 3 <> 0 && n % 5 <> 0 && n % 7 <> 0
-    then
-        string_of_int n
-    else
-        (if n % 3 = 0 then literal_to_string "Pling" else literal_to_string "")
-        ^ (if n % 5 = 0 then literal_to_string "Plang" else literal_to_string "")
-        ^ (if n % 7 = 0 then literal_to_string "Plong" else literal_to_string "")
+val raindrop_return_any_sound: (n:native_int) -> Lemma (ensures S.length (raindrop n) > 0)
+let raindrop_return_any_sound n = match of_int n with
+    | n when n % 3 <> 0 && n % 5 <> 0 && n % 7 <> 0 -> ()
+    | n -> empty_string_length_is_zero "";
+            not_empty_string_length_is_pos "Pling";
+            not_empty_string_length_is_pos "Plang";
+            not_empty_string_length_is_pos "Plong"
